save

WellFormedness.v
@@ -1,1 +1,106 @@
 From TL Require Import Identifier Environment Imperative Types Augmented.
+
+Definition wf_mem (m : state) (Γ : typenv) : Prop :=
+  (forall x u, m x = Some u -> exists l, Γ x = Some l)
+  /\
+  (forall x l, Γ x = Some l -> exists u, m x = Some u).
+
+Lemma update_preserves_wf_mem: forall m Γ x l v,
+    wf_mem m Γ ->
+    Γ x = Some l ->
+    wf_mem (update_env m x v) Γ.
+Proof.
+Admitted.
+
+(* - m is well-formed w.r.t. Γ
+   - c is well-typed under Γ and pc (if c is not stop)
+ *)
+Definition wf_cfg (cfg : config) (Γ : typenv) (pc: level): Prop :=
+  match cfg with
+  | Config c m => wf_mem m Γ /\ (c <> STOP -> -{ Γ, pc ⊢ c }-)
+  end.
+
+Notation  "'={' Γ ',' pc '⊢' cfg '}='" := 
+  (wf_cfg cfg Γ pc ) (at level 40).
+
+Theorem preservation_wf_cfg: forall Γ pc cfg cfg',
+    ={ Γ, pc ⊢ cfg }= ->
+    cfg ⇒ cfg' ->
+    ={ Γ, pc ⊢ cfg'}= .
+Proof.
+
+  intros Γ pc [c m] [c' m'].
+  intros [H_wf_mem H_wf_cmd] H_step.
+
+  remember (Config c m) as cfg0 eqn:Heq0.
+  remember (Config c' m') as cfg1 eqn:Heq1.
+
+  (* to make the I.H. stronger, we need to *)
+  revert c m c' m' Heq0 Heq1 H_wf_mem H_wf_cmd.
+
+  induction H_step;
+  intros cc mm cc' mm' Heq0 Heq1 H_wf_mem H_wf_cmd;
+  inversion Heq0; inversion Heq1; subst; simpl in *.
+
+  (* step_skip *)
+  - unfold wf_cfg. split.
+    + apply H_wf_mem.
+    + contradiction.
+  (* step_assign *)
+  - unfold wf_cfg. split.
+    + assert (H_assign_neq_stop : x ::= e <> STOP) 
+        by apply assign_neq_stop.
+      specialize (H_wf_cmd H_assign_neq_stop) as H_wf_cmd'.
+      inversion H_wf_cmd'.
+      apply update_preserves_wf_mem with (l:=lx).
+      assumption.
+      assumption.
+    + contradiction.
+  (* step_seq1 *)
+  - assert (H_seq_neq_stop : (c1 ;; c2) <> STOP) by apply seq_neq_stop.
+    (* build C1_well_typed *)
+    specialize (H_wf_cmd H_seq_neq_stop) as H_wf_cmd'.
+    inversion H_wf_cmd'.
+    assert (C1_well_typed : c1 <> STOP -> -{ Γ, pc ⊢ c1 }-).
+      { 
+        destruct (eq_cmd_stop_dec c1) as [Heq | Hneq].
+        { contradiction. }
+        { intro. apply H4. }
+      }
+    (* use I.H. *)
+    assert (config_eq_1 : 〈 c1, mm 〉 = 〈 c1, mm 〉) by reflexivity.
+    assert (config_eq_2 : 〈 c1', mm' 〉 = 〈 c1', mm' 〉) by reflexivity.
+    specialize IHH_step with (c:=c1) (m:=mm) (c':=c1') (m':=mm').
+    specialize (IHH_step config_eq_1 config_eq_2 H_wf_mem C1_well_typed) as [IH1 IH2].
+    (* use IH1 IH2 *)
+    split.
+    + apply IH1.
+    + intro. apply T_Seq. apply IH2 in H. assumption. assumption.
+  (* step_seq2 *)
+  - assert (H_seq_neq_stop : (c1 ;; cc') <> STOP) by apply seq_neq_stop.
+    (* build C1_well_typed *)
+    specialize (H_wf_cmd H_seq_neq_stop) as H_wf_cmd'.
+    inversion H_wf_cmd'.
+    assert (C1_well_typed : c1 <> STOP -> -{ Γ, pc ⊢ c1 }-).
+      { 
+        destruct (eq_cmd_stop_dec c1) as [Heq | Hneq].
+        { contradiction. }
+        { intro. apply H3. }
+      }
+    (* use I.H. *)
+    assert (config_eq_1 : 〈 c1, mm 〉 = 〈 c1, mm 〉) by reflexivity.
+    assert (config_eq_2 : 〈 STOP, mm' 〉 = 〈 STOP, mm' 〉) by reflexivity.
+    specialize IHH_step with (c:=c1) (m:=mm) (c':=STOP) (m':=mm').
+    specialize (IHH_step config_eq_1 config_eq_2 H_wf_mem C1_well_typed) as [IH1 IH2].
+    (* use IH1 IH2 *)
+    split.
+    + apply IH1.
+    + destruct (eq_cmd_stop_dec cc') as [Heq | Hneq].
+        { contradiction. }
+        { intro. apply H4. }
+  (* step_if1 *)
+  - 
+
+
+      
+      
